Checks/Bls12381G1AddSourceFpMulStep0.lean
@@ -7,7 +7,7 @@ namespace Challenge.Bls12381G1Add.Reference.Proofs.SourceSemantics
 open YulSemantics YulSemantics.EVM
 
 example (ahi alo bhi blo : U256) (yst : EvmState) :
-    Interp.execStmt Challenge.EvmProof.modexpExec 65 fpMulFuns
+    Interp.execStmt Challenge.EvmProof.modexpExec 65 fpMulBodyFuns
       (fpMulInitialEnv ahi alo bhi blo) yst fpMulStmt0 =
     .ok (fpMulProductEnv ahi alo bhi blo, yst, .normal) :=
   exec_fpMulStmt0 ahi alo bhi blo yst
